refactor Fin

Lambda/Fin.lean
@@ -1,22 +1,65 @@
-inductive Fin' : Nat → Type where
-| fz : Fin' (n + 1)
-| fs : Fin' n → Fin' (n + 1)
+namespace List
 
-def Fin'.ofNat : ∀ {m} (n), n < m → Fin' m
-| _ + 1, 0, _ => fz
-| _ + 1, (n + 1), h => fs (Fin'.ofNat n (Nat.le_of_succ_le_succ h))
+variable {α : Type u}
 
-inductive Vec (α : Type u) : Nat → Type u where
-| nil : Vec α 0
-| cons : α → Vec α n → Vec α (n + 1)
+inductive Fin : α → List α → Type u
+| fz : List.Fin x (x :: l)
+| fs : List.Fin x l → List.Fin x (y :: l)
+infix:60 " ∈' " => Fin
 
-notation "[]ᵥ" => Vec.nil
-infixr:55 " ∷ᵥ " => Vec.cons
+def Fin.ofNatType (n : Nat) : Type u :=
+  ∀ {x l}, ofNatTypeAux n x (x :: l)
+where
+  ofNatTypeAux : Nat → α → List α → Type u
+  | 0, x, l => x ∈' l
+  | m + 1, x, l => ∀ {y}, ofNatTypeAux m x (y :: l)
 
-instance : EmptyCollection (Vec α 0) := ⟨[]ᵥ⟩
-@[simp] def Vec.add (v : Vec α n) (x : α) := x ∷ᵥ v
-infixl:55 ",' " => Vec.add
+def Fin.ofNat (n : Nat) : @Fin.ofNatType α n :=
+  ofNatAux n fz
+where
+  ofNatAux {x : α} {l : List α} :
+    (n : Nat) → x ∈' l → ofNatType.ofNatTypeAux n x l
+  | 0 => λ h => h
+  | n + 1 => λ h {_} => (ofNatAux n (fs h))
 
-def Vec.get : Vec α n → Fin' n → α
-| a ∷ᵥ _, Fin'.fz => a
-| _ ∷ᵥ v, Fin'.fs x => v.get x
+def Fin.mem : x ∈' l → x ∈ l
+| fz => Mem.head _
+| fs h => Mem.tail _ (mem h)
+
+def Fin.fin : x ∈' l → _root_.Fin l.length
+| fz => ⟨0, Nat.zero_lt_succ _⟩
+| fs h => match fin h with
+          | ⟨n, h⟩ => ⟨n + 1, Nat.succ_le_succ h⟩
+
+theorem Fin.fin_get (h : x ∈' l) : l.get (fin h) = x := by
+  induction h with
+  | fz => rfl
+  | fs h ih => simp [get, ←ih]
+
+end List
+
+export List.Fin (fz fs)
+
+
+-- inductive Fin' : Nat → Type where
+-- | fz : Fin' (n + 1)
+-- | fs : Fin' n → Fin' (n + 1)
+
+-- def Fin'.ofNat : ∀ {m} (n), n < m → Fin' m
+-- | _ + 1, 0, _ => fz
+-- | _ + 1, (n + 1), h => fs (Fin'.ofNat n (Nat.le_of_succ_le_succ h))
+
+-- inductive Vec (α : Type u) : Nat → Type u where
+-- | nil : Vec α 0
+-- | cons : α → Vec α n → Vec α (n + 1)
+
+-- notation "[]ᵥ" => Vec.nil
+-- infixr:55 " ∷ᵥ " => Vec.cons
+
+-- instance : EmptyCollection (Vec α 0) := ⟨[]ᵥ⟩
+-- @[simp] def Vec.add (v : Vec α n) (x : α) := x ∷ᵥ v
+-- infixl:55 ",' " => Vec.add
+
+-- def Vec.get : Vec α n → Fin' n → α
+-- | a ∷ᵥ _, Fin'.fz => a
+-- | _ ∷ᵥ v, Fin'.fs x => v.get x
